{
 "cells": [
  {
   "cell_type": "raw",
   "id": "057ec963-6e61-4dcb-a220-dc4b3dfb83a8",
   "metadata": {},
   "source": [
    "Question 1.Find the val%e of T(2) for the rec%rrence relation T(n) = 3T(n-1) + 12n, given that T(0)=5.\n",
    "\n",
    "\n",
    "This recurrence relation (T(n) = 3T(n-1) + 12n) defines a function where the value of (T(n)) depends on the previous value (T(n-1))\n",
    "and the input  (n ).\n",
    "\n",
    "To find  (T(2) ), we will use the given recurrence relation and the base case (T(0) = 5).\n",
    "\n",
    "Given:\n",
    "(T(0) = 5)\n",
    "\n",
    "Using the recurrence relation (T(n) = 3T(n-1) + 12n):\n",
    "\n",
    "(T(1) = 3T(1-1) + 12(1) = 3T(0) + 12 = 3 times 5 + 12 = 15 + 12 = 27)\n",
    "\n",
    "(T(2) = 3T(2-1) + 12(2) = 3T(1) + 24 = 3 times 27 + 24 = 81 + 24 = 105)\n",
    "\n",
    "So, the value of (T(2)) for the given recurrence relation and base case is (105)."
   ]
  },
  {
   "cell_type": "raw",
   "id": "941cf575-e81e-42dc-8962-7ff5722396a7",
   "metadata": {},
   "source": [
    "Question 2. Given a recurrence relation, solve it using the substitution method:\n",
    "a. T(n) = T(n-1) + c\n",
    "\n",
    "\n",
    "=>  Sure, to solve the recurrence relation (T(n) = T(n-1) + c) using the substitution method,\n",
    "we will try to find a pattern and derive a closed-form expression for (T(n)).\n",
    "\n",
    "Given:\n",
    "(T(n) = T(n-1) + c)\n",
    "\n",
    "Let's start with the base case:\n",
    "\n",
    "(T(1) = T(1-1) + c = T(0) + c)\n",
    "\n",
    "Now, let's try to establish a pattern by expanding (T(2), T(3)) and so on:\n",
    "\n",
    "(T(2) = T(2-1) + c = T(1) + c = (T(0) + c) + c = T(0) + 2c)\n",
    "\n",
    "(T(3) = T(3-1) + c = T(2) + c = (T(0) + 2c) + c = T(0) + 3c)\n",
    "\n",
    "From this pattern, we can generalize:\n",
    "\n",
    "(T(n) = T(0) + nc)\n",
    "\n",
    "So, in terms of (n) and the constant (c), the solution to the recurrence relation (T(n) = T(n-1) + c) using the substitution method is:\n",
    "\n",
    "[T(n) = T(0) + nc]\n",
    "\n",
    "This solution provides a closed-form expression for (T(n)) in terms of the initial condition (T(0)) and the constant (c), where \n",
    "(n) is the number of steps or iterations.\n",
    "\n",
    "\n",
    "\n",
    "\n",
    "\n",
    "\n",
    "\n",
    "\n",
    "b. (T(n) = 2T(n/2) + n)\n",
    "\n",
    "Let's assume (n = 2^k) for some non-negative integer (k). Then, (n/2 = 2^{k-1}).\n",
    "\n",
    "[T(2^k) = 2T(2^{k-1}) + 2^k]\n",
    "\n",
    "Let (S(k) = T(2^k)). Then the equation becomes:\n",
    "\n",
    "[S(k) = 2S(k-1) + 2^k]\n",
    "\n",
    "Now, let's solve this recurrence relation by iteratively substituting:\n",
    "\n",
    "[S(k) = 2S(k-1) + 2^k]\n",
    "[= 2(2S(k-2) + 2^{k-1}) + 2^k]\n",
    "[= 2^2S(k-2) + 2^k + 2^k]\n",
    "[= 2^2S(k-2) + 2.2^k]\n",
    "\n",
    "Continuing this process, after (m) steps, we get:\n",
    "\n",
    "[S(k) = 2^mS(k-m) + m.2^k]\n",
    "\n",
    "When (k = m), (S(k-m) = S(0)) (the base case).\n",
    "\n",
    "So, when (k = m = log_2 n), we get:\n",
    "\n",
    "[S(log_2 n) = 2^{log_2 n}S(0) + log_2 n.2^{log_2 n}]\n",
    "[= nS(0) + nlog_2 n]\n",
    "\n",
    "Therefore, (T(n) = nT(1) + nlog_2 n = nT(1) + nlog ) (as log_2 n = log n log 2)).\n",
    "\n",
    "\n",
    "\n",
    "\n",
    "\n",
    "c. (T(n) = 2T(n/2) + c)\n",
    "\n",
    "Following a similar process as before:\n",
    "\n",
    "Let's assume  (n = 2^k ) for some non-negative integer  (k ).\n",
    "\n",
    " [T(2^k) = 2T(2^{k-1}) + c ]\n",
    "\n",
    "Let  (S(k) = T(2^k) ). Then the equation becomes:\n",
    "\n",
    " [S(k) = 2S(k-1) + c ]\n",
    "\n",
    "Solving this recurrence relation follows a similar pattern to the first one, and after  (k =  log_2 n ) steps:\n",
    "\n",
    " [S( log_2 n) = nT(1) + c  cdot  log_2 n = nT(1) + c  cdot  log n ]\n",
    " \n",
    " \n",
    " \n",
    " \n",
    "\n",
    "d.  (T(n) = T(n/2) + c )\n",
    "\n",
    "Let's assume  (n = 2^k ) for some non-negative integer  (k ).\n",
    "\n",
    " [T(2^k) = T(2^{k-1}) + c ]\n",
    "\n",
    "Let  (S(k) = T(2^k) ). Then the equation becomes:\n",
    "\n",
    " [S(k) = S(k-1) + c ]\n",
    "\n",
    "After  (k =  log_2 n ) steps:\n",
    "\n",
    " [S( log_2 n) = S(0) + c  cdot  log_2 n = T(1) + c  cdot  log n ]\n",
    "\n",
    "These solutions provide closed-form expressions for  (T(n) ) in terms of the initial conditions and the specific patterns observed in each recurrence relation."
   ]
  },
  {
   "cell_type": "raw",
   "id": "3c606173-5cd6-406f-9d13-fb699de77420",
   "metadata": {},
   "source": [
    "Question 3. Given a recurrence relation, solve it using the recursive tree approach:\n",
    "a. T(n) = 2T(n-1) +1\n",
    "b. T(n) = 2T(n/2) + n\n",
    "\n",
    "\n",
    "\n",
    "Let's solve these recurrence relations using the recursive tree approach:\n",
    "\n",
    "### a.  (T(n) = 2T(n-1) + 1 )\n",
    "\n",
    "This recurrence relation implies that at each step, the function  (T(n) ) is dependent on twice the value of  (T ) at the previous step ( (T(n-1) )) plus 1.\n",
    "\n",
    "To visualize this using a recursive tree:\n",
    "\n",
    "```\n",
    "                           T(n)\n",
    "                          /    \\\n",
    "                   T(n-1)+1   T(n-1)+1\n",
    "                     /          /  \n",
    "            T(n-2)+1 T(n-2)+1 T(n-2)+1 T(n-2)+1\n",
    "               . . .\n",
    "```\n",
    "\n",
    "The tree shows that at each level, there are two branches, each contributing 1. This forms a binary tree with a depth of  (n ) levels.\n",
    "\n",
    "If we sum up the number of nodes at each level of this tree, we get a geometric series:\n",
    "\n",
    " [ text{Total number of nodes} = 1 + 2 + 4 +  dots + 2^n = 2^{n+1} - 1 ]\n",
    "\n",
    "Therefore, the time complexity of this recurrence relation is exponential, specifically  (O(2^n) ).\n",
    "\n",
    "### b.  (T(n) = 2T(n/2) + n )\n",
    "\n",
    "This recurrence relation represents a divide-and-conquer algorithm where the problem is divided into two equal parts at each step, and the solution involves the sum of the problem size ( (n )).\n",
    "\n",
    "The recursive tree for this relation would look like:\n",
    "\n",
    "```\n",
    "                        T(n)\n",
    "                      /      \\\n",
    "                  T(n/2)+n  T(n/2)+n\n",
    "                   /          /  \n",
    "              T(n/4)+n T(n/4)+n ...\n",
    "```\n",
    "\n",
    "Here, at each level, the value of  (n ) reduces by half (as  (n/2 )) at each subsequent level. The depth of this tree would be  ( log n ) because the problem size is halved at each step.\n",
    "\n",
    "To calculate the total work done, we sum the work at each level of the tree. At level  (i ), there are  (2^i ) nodes, each contributing  (n/2^i ). Therefore, the total work is:\n",
    "\n",
    " [T(n) = n log n + n left( log n - 1 right) +  dots + n = O(n  log n) ]\n",
    "\n",
    "So, the time complexity of this recurrence relation  (T(n) = 2T(n/2) + n ) is  (O(n  log n) )."
   ]
  },
  {
   "cell_type": "code",
   "execution_count": null,
   "id": "2969dbe6-d671-4428-a6d6-ca2c87d770cb",
   "metadata": {},
   "outputs": [],
   "source": []
  }
 ],
 "metadata": {
  "kernelspec": {
   "display_name": "Python 3 (ipykernel)",
   "language": "python",
   "name": "python3"
  },
  "language_info": {
   "codemirror_mode": {
    "name": "ipython",
    "version": 3
   },
   "file_extension": ".py",
   "mimetype": "text/x-python",
   "name": "python",
   "nbconvert_exporter": "python",
   "pygments_lexer": "ipython3",
   "version": "3.10.8"
  }
 },
 "nbformat": 4,
 "nbformat_minor": 5
}
